lib/Free.fst
@@ -1,11 +1,18 @@
 module Free
 
-(** Sum of two command types.
-    Commands are indexed types (Type0 -> Type) parameterizing the free monad. *)
+(** Sum of two command types (within one channel of the free monad).
+    Commands are indexed types (Type -> Type) parameterizing the free monad.
+    Note that the two summands must have the same index universe: to mix
+    commands whose result types live in different universes, put them on
+    different channels of the free monad below. *)
 noeq
 type cmd_sum (cmd1 cmd2 : Type -> Type) : Type -> Type =
 | CmdL : #r:Type -> cmd1 r -> cmd_sum cmd1 cmd2 r
 | CmdR : #r:Type -> cmd2 r -> cmd_sum cmd1 cmd2 r
+
+(** The empty command type: instantiates an unused channel. *)
+noeq
+type empty_cmds : Type u#0 -> Type u#0 =
 
 (** Sum of two event types.
     Events are plain types parameterizing the hist monad. *)
@@ -14,36 +21,48 @@ type event_sum (ev1 ev2 : Type) =
 | EvL : ev1 -> event_sum ev1 ev2
 | EvR : ev2 -> event_sum ev1 ev2
 
+(** The free monad has two command channels with independent universes.
+    Universes of a datatype are computed per constructor and joined with
+    max, so Call1 and Call2 can quantify their result types at different
+    universes. This allows mixing commands whose results live in different
+    universes without universe-lifting wrappers: each command type goes on
+    the channel matching its index universe. *)
 noeq
-type free (cmd : Type u#i -> Type u#e) (a:Type u#a) : Type u#(max (1 + i) (max a e)) =
-| Call : #r:Type u#i -> cmd r -> cont:(r -> free cmd a) -> free cmd a
-| Return : a -> free cmd a
+type free (cmd1 : Type u#i -> Type u#j) (cmd2 : Type u#f -> Type u#g) (a:Type u#a)
+  : Type u#(max (1 + i) (max (1 + f) (max j (max g a)))) =
+| Call1 : #r:Type u#i -> cmd1 r -> cont:(r -> free cmd1 cmd2 a) -> free cmd1 cmd2 a
+| Call2 : #r:Type u#f -> cmd2 r -> cont:(r -> free cmd1 cmd2 a) -> free cmd1 cmd2 a
+| Return : a -> free cmd1 cmd2 a
 
-val free_return : #cmd:(Type u#i -> Type u#e) -> #a:Type u#a -> x:a -> free cmd a
-let free_return #cmd #a (x:a) : free cmd a =
+val free_return : #cmd1:(Type u#i -> Type u#j) -> #cmd2:(Type u#f -> Type u#g) -> #a:Type u#a -> x:a -> free cmd1 cmd2 a
+let free_return #cmd1 #cmd2 #a (x:a) : free cmd1 cmd2 a =
   Return x
 
-val free_bind : #cmd:(Type u#i -> Type u#e) -> #a:Type u#a -> #b:Type u#b -> l:free cmd a -> k:(a -> free cmd b) -> free cmd b
+val free_bind : #cmd1:(Type u#i -> Type u#j) -> #cmd2:(Type u#f -> Type u#g) -> #a:Type u#a -> #b:Type u#b -> l:free cmd1 cmd2 a -> k:(a -> free cmd1 cmd2 b) -> free cmd1 cmd2 b
 let rec free_bind
-  #cmd #a #b
-  (l : free cmd a)
-  (k : a -> free cmd b) :
-  free cmd b =
+  #cmd1 #cmd2 #a #b
+  (l : free cmd1 cmd2 a)
+  (k : a -> free cmd1 cmd2 b) :
+  free cmd1 cmd2 b =
   match l with
   | Return x -> k x
-  | Call op fnc ->
-      Call op (fun i ->
+  | Call1 op fnc ->
+      Call1 op (fun i ->
+        free_bind (fnc i) k)
+  | Call2 op fnc ->
+      Call2 op (fun i ->
         free_bind (fnc i) k)
 
-val free_map : #cmd:(Type u#i -> Type u#e) -> #a:Type u#a -> #b:Type u#b -> l:free cmd a -> k:(a -> b) -> Tot (free cmd b)
+val free_map : #cmd1:(Type u#i -> Type u#j) -> #cmd2:(Type u#f -> Type u#g) -> #a:Type u#a -> #b:Type u#b -> l:free cmd1 cmd2 a -> k:(a -> b) -> Tot (free cmd1 cmd2 b)
 let free_map
-  #cmd #a #b
-  (l : free cmd a)
+  #cmd1 #cmd2 #a #b
+  (l : free cmd1 cmd2 a)
   (k : a -> b) :
-  Tot (free cmd b) =
+  Tot (free cmd1 cmd2 b) =
   free_bind l (fun x -> free_return (k x))
 
 let free_codomain_ordering
-  #cmd #a
-  (x:(free cmd a){Call? x}) :
-  Lemma (forall r. Call?.cont x r << x) = ()
+  #cmd1 #cmd2 #a
+  (x:(free cmd1 cmd2 a){Call1? x \/ Call2? x}) :
+  Lemma ((Call1? x ==> (forall r. Call1?.cont x r << x)) /\
+         (Call2? x ==> (forall r. Call2?.cont x r << x))) = ()
